Modify the front-end to produce code mostly consistent with the following grammar prefered by the back-end (except for the shifting operations): let r range over register names (r0,r1,r2,etc), m range over memory locations (m0,m1,m2,etc), f over function names, i over natural numbers (<32) and w over 8-bit word constants.
 p    ::=  let r = exp in p
 | let m = r in p
 | let (v,v,...,v) = f (v,v,...,v) in p
 | if g then p else p
 | (v,v,...,v)  |  f (v,v,...,v)

 v    ::=  r  |  m
 g    ::=  ~ g  |  r cmp mode  |  r && mode = 0w
 cmp  ::=  =  |  <  |  <+  |  <=  |  <=+
 exp  ::=  m  |  mode  |  ~ mode  |  r op mode  |  r * r
 op   ::=  + | - | && | ?? | !!
 mode ::=  w  |  r  |  r << i  |  r >> i  |  r >>> i

examples/dev/sw2/basic.sig
@@ -2,9 +2,12 @@ signature basic =
 sig
   include Abbrev
   val is_word_literal : term -> bool
+  val is_literal : term -> bool
+  val is_8bit_literal : term -> bool
   val is_atomic : term -> bool 
   val is_num_arithop : term -> bool 
   val is_word_arithop : term -> bool 
+  val is_mult_op : term -> bool
   val is_num_cmpop : term -> bool 
   val is_word_cmpop : term -> bool 
   val is_word_bitwiseop : term -> bool
